lean4/Automaton/NFA/Basic.lean
@@ -1,5 +1,6 @@
 import Mathlib.Data.Set.Lattice
 import Automaton.Language.Basic
+import Automaton.Finset.Basic
 
 /-!
   This file contains the definition of NFA as well as a few fundemantal operations
@@ -9,40 +10,39 @@ import Automaton.Language.Basic
 namespace NFA
 
 structure NFA (σ : Type _) where
-  q : Type _        -- states
-  init : q          -- initial state
-  fs : Set q        -- accepting states
-  δ : q → σ → Set q -- transition function
-  [d : DecidablePred fs]
+  q : Finset Nat        -- states
+  init : Nat          -- initial state
+  fs : Finset Nat       -- accepting states
+  δ : Nat → σ → Finset Nat -- transition function
 
 variable {σ : Type _} (t : NFA σ)
 
+
 -- one step in the operation of NFA, consuming one character
 -- take the union of all sets of states reachable from current set of states
-def δ_step  (q : Set t.q) (e : σ) : Set t.q := ⋃₀ {t.δ a e | a ∈ q}
+def δ_step  (q : Finset Nat) (e : σ) : Finset Nat := q.biUnion (fun n => t.δ n e)
 
 -- δ* function for NFA
 -- returns set of states reached after inputting a word
-def δ_star : (w : word σ) → Set t.q 
+def δ_star : (w : word σ) → Finset Nat
   | [] => {t.init}
   | e :: es => δ_step t (δ_star es) e 
 
 -- Whether a word is in the language that the NFA accepts
 def nfa_accepts (w : word σ) : Prop := by
-  have δ_fs : Set t.q := δ_star t w
-  have i := Set.inter δ_fs t.fs 
-  exact i.Nonempty
+  have inter : Finset Nat := (δ_star t w) ∩ t.fs
+  exact inter.Nonempty
 
 -- nfa accepts nil iff init is final
 theorem nfa_accepts_nil_iff_final : nfa_accepts t [] ↔ t.init ∈ t.fs := by
   apply Iff.intro
-  · intro h
-    dsimp [nfa_accepts, δ_star ] at h
-    apply (Iff.mp Set.singleton_inter_nonempty)
-    exact h
+  · intro ne
+    dsimp [nfa_accepts, δ_star ] at ne
+    apply Finset.nonempty_inter_singleton_imp_in
+    exact ne
   · intro e
-    dsimp [nfa_accepts]
-    apply (Iff.mpr Set.singleton_inter_nonempty)
-    exact e
-    
+    dsimp [nfa_accepts,δ_star]
+    rw [Finset.singleton_inter_of_mem e]
+    exact (Finset.singleton_nonempty t.init)
+
 end NFA
