lean4/Automaton/DFA/Examples.lean
@@ -13,22 +13,16 @@ def trans_fun : Nat → Char → Nat
   | 1 , '1' => 1
   | _ , _ => 2
 
--- 1 is the only final state
-def fin_states : Set Nat := fun n => n = 1
 
--- the membership of a set of fin states must be decidable for the language 
--- to be decidable
-instance : DecidablePred (fin_states) := by
-  intro n
-  dsimp [fin_states]
-  cases n with
-  | zero => apply Decidable.isFalse; trivial
-  | succ n => cases n with
-    | zero => apply Decidable.isTrue; trivial
-    | succ n => apply Decidable.isFalse; simp; apply Nat.succ_ne_zero
+
+def states : Finset Nat := {0 , 1 , 2}
+
+-- 1 is the only final state
+def fin_states : Finset Nat := {1}
+
 
 -- accepts all words that end with '1'
-def last_is_one : DFA Char := {q := Nat , init := 0 , fs := fin_states , δ := trans_fun}
+def last_is_one : DFA Char := {q := states , init := 0 , fs := fin_states , δ := trans_fun}
 
 -- words are consumed backwwards, see definition of δ_star
 def w1 : word Char := [ '1','0' ]
