lean4/Automaton/DFA/ToNFA.lean
@@ -1,11 +1,12 @@
 import Automaton.DFA.Basic
 import Automaton.NFA.Basic
+import Automaton.Finset.Basic
 
 /-!
   This file contains conversion from DFA to NFA `dfa_to_nfa`
   Proves several things about such converted automata such as equality of δ_star function
   Contains a definition of what equality between NFA and DFA means
-  Then asserts that the converted DFA fulfills this property
+  Then asserts that the converted DFA fulfills is property
 -/
 
 open DFA NFA
@@ -18,15 +19,14 @@ variable {σ : Type _} (td sd : DFA σ) (tn sn : NFA σ)
 def dfa_nfa_eq : Prop := ∀ w : word σ , nfa_accepts tn w ↔ dfa_accepts td w
 
 -- to convert into nfa δ, just create singleton for each state
-def dfa_δ_to_nfa_δ : td.q → σ → Set td.q := λ q s => {td.δ q s}
+def dfa_δ_to_nfa_δ : Nat → σ → Finset Nat := λ q e => {td.δ q e}
 
 -- conversion from nfa to dfa
 def dfa_to_nfa : NFA σ := by
   exact {q := td.q , init := td.init , fs := td.fs , δ := dfa_δ_to_nfa_δ td : NFA σ}
 
 -- the initial state in NFA is same as in the original DFA
-theorem dfa_to_nfa_eq_init : td.init = (dfa_to_nfa td).init := by
-  dsimp [dfa_to_nfa]
+theorem dfa_to_nfa_eq_init : td.init = (dfa_to_nfa td).init := by dsimp [dfa_to_nfa]
 
 -- the final states of the converted dfa are the same
 theorem dfa_to_nfa_eq_final : td.fs = (dfa_to_nfa td).fs := by dsimp[dfa_to_nfa]
@@ -35,7 +35,9 @@ theorem dfa_to_nfa_eq_final : td.fs = (dfa_to_nfa td).fs := by dsimp[dfa_to_nfa]
 theorem dfa_to_nfa_eq_δ_star  (w : word σ) : {DFA.δ_star td w} = NFA.δ_star (dfa_to_nfa td) w := by
   induction w with
   | nil => dsimp [DFA.δ_star,NFA.δ_star]; rw [←dfa_to_nfa_eq_init]
-  | cons a as h => dsimp [DFA.δ_star,NFA.δ_star]; rw [←h]; simp [δ_step,dfa_to_nfa,dfa_δ_to_nfa_δ]
+  | cons a as h => dsimp [DFA.δ_star,NFA.δ_star] 
+                   rw [←h];
+                   simp [δ_step,dfa_to_nfa,dfa_δ_to_nfa_δ, δ']              
 
 -- converted dfa accepts the same language as the original dfa
 theorem dfa_to_nfa_eq : dfa_nfa_eq td (dfa_to_nfa td) := by
@@ -46,14 +48,16 @@ theorem dfa_to_nfa_eq : dfa_nfa_eq td (dfa_to_nfa td) := by
     simp [nfa_accepts] at h
     simp [dfa_accepts]
     rw [←(dfa_to_nfa_eq_δ_star td w)] at h
-    apply (Iff.mp Set.singleton_inter_nonempty)
+    apply Finset.nonempty_inter_singleton_imp_in
     exact h
   · intro h
     simp [nfa_accepts]
     simp [dfa_accepts] at h
-    rw [←(dfa_to_nfa_eq_δ_star td w)] 
-    apply (Iff.mpr Set.singleton_inter_nonempty)
-    exact h
+    rw [←(dfa_to_nfa_eq_δ_star td w)]
+    simp [dfa_to_nfa]
+    rw [Finset.singleton_inter_of_mem h]
+    exact (Finset.singleton_nonempty (DFA.δ_star td w))
+
 
 end ToNFA
 
