lean4/Automaton/Finset/Basic.lean
@@ -1,0 +1,15 @@
+import Mathlib.Data.Finset.Basic
+
+
+namespace Finset
+
+theorem nonempty_inter_singleton_imp_in {α : Type _} [DecidableEq α] (e : α) (es : Finset α) : 
+  Finset.Nonempty ({e} ∩ es) → e ∈ es := by
+    intro ne
+    have h₁ : e ∉ es → {e} ∩ es = ∅ := Finset.singleton_inter_of_not_mem
+    have h₂ := Not.imp_symm h₁
+    apply h₂
+    apply (Iff.mp Finset.nonempty_iff_ne_empty)
+    exact ne
+
+end Finset
